heap equivalence

src/Safety.v
@@ -1,17 +1,75 @@
 Require Import Gc.Language Gc.Gc.
 
+Require Import CpdtTactics.
+
+Definition equiv' (s1 s2: state) : Prop :=
+  forall v p1 address p1' k i,
+      roots_maps (roots s1) v p1 ->
+      addresses (heap s1) p1 address p1' ->
+      heap_maps (heap s1) p1' k (Int i) ->
+      exists p2 p2',
+        roots_maps (roots s2) v p2 /\
+        addresses (heap s2) p2 address p2' /\
+        heap_maps (heap s2) p2' k (Int i).
+
+Definition equiv (s1 s2: state) : Prop :=
+  (output s1 = output s2) /\ equiv' s1 s2 /\ equiv' s2 s1.
+
+Lemma equiv_refl : forall s1, equiv s1 s1.
+  intros.
+  unfold equiv.
+  split. reflexivity.
+  split ;
+    unfold equiv' ;
+    intros ;
+    exists p1, p1';
+    auto.
+Qed.
+
+Lemma equiv_symm : forall s1 s2, equiv s1 s2 -> equiv s2 s1.
+  intros.
+  unfold equiv in *.
+  crush.
+Qed.
+
+Ltac destructo :=
+  repeat match goal with
+         | [H : _ /\ _ |- _] => destruct H
+         | [H : exists _, _|- _] => destruct H
+         end.
+
+Lemma equiv_trans : forall s1 s2 s3, equiv s1 s2 -> equiv s2 s3 -> equiv s1 s3.
+Proof.
+  intros.
+  unfold equiv in *.
+  destructo.
+  split. crush.
+  clear H H0.
+  split.
+  * unfold equiv'.
+    intros.
+    specialize (H3 v p1 address p1' k i).
+    intuition.
+    destructo.
+    eapply H1.
+    apply H3.
+    apply H6.
+    apply H7.
+  * unfold equiv'.
+    intros.
+    specialize (H2 v p1 address p1' k i).
+    intuition.
+    destructo.
+    eapply H4.
+    apply H2.
+    apply H6.
+    apply H7.
+Qed.
+
 (* All integers reachable from the same variable, address, and index. *)
 Theorem gc_safety :
-  forall st st' p p' v address k i,
-    roots_maps (roots st) v p ->
-    addresses (heap st) p address p' ->
-    heap_maps (heap st) p' k (Int i) ->
-    gc st = st' ->
-    (exists p'' p''', 
-      roots_maps (roots st') v p'' /\
-      addresses (heap st') p'' address p''' /\
-      heap_maps (heap st') p''' k (Int i)
-    )
+  forall st st',
+    equiv st st'
 .
 Proof.
 Admitted.
